Fix params

frodo/code/params-976-cSHAKEx64/Hacl.Impl.Frodo.Params.fst
@@ -7,4 +7,4 @@ include Frodo.Params
 
 let cshake_frodo = Hacl.Keccak.cshake256_frodo
 
-let frodo_gen_matrix = Hacl.Impl.Frodo.Gen.frodo_gen_matrix_cshake4x
+let frodo_gen_matrix = Hacl.Impl.Frodo.Gen.frodo_gen_matrix_cshake_4x
