frodo/spec/params-64-cSHAKE/Frodo.Params.fst
@@ -1,0 +1,25 @@
+module Frodo.Params
+
+open Lib.IntTypes
+
+unfold let params_n = size 64
+
+unfold let params_logq = size 15
+
+unfold let params_extracted_bits = size 2
+
+unfold let crypto_bytes = size 16
+
+unfold let cdf_table_len = size 12
+
+unfold let cdf_list: list uint16 = 
+  [u16 4727;  u16 13584; u16 20864; u16 26113; u16 29434; u16 31278;
+   u16 32176; u16 32560; u16 32704; u16 32751; u16 32764; u16 32767]
+
+unfold let bytes_seed_a = size 16
+
+unfold let params_nbar = size 8
+
+unfold let frodo_prf_spec = Spec.Frodo.Keccak.cshake128_frodo
+
+unfold let frodo_gen_matrix = Spec.Frodo.Gen.frodo_gen_matrix_cshake
